src/base2.lean
@@ -1,49 +1,106 @@
+import tactic
 import algebra algebra.group algebra.group.defs logic.relation order.lexicographic
 import data
-universes u v variables (α β : Type*)
+universes u v variables {α β : Type*}
+def nat.decr : ℕ → ℕ | 0 := 0 | (n+1) := n
+def elementary {I V : Type} [decidable_eq I] [add_monoid V] (i : I) (v : V) := λ j, if i = j then v else 0
+instance unit.has_top : has_top unit := ⟨()⟩
+inductive reduces {α : Type u} (r : α → α → Prop) : α → α → Type u
+| refl {s} : reduces s s
+| tail {a b c} : r a b → reduces b c → reduces a c
 structure iter (σ I V : Type*) :=
-  (δ : function.End σ) (ι : σ → I) (ν : σ → V) (ready : σ → bool)
-structure stream (σ I V : Type*) := (iter : iter σ I V) (q : σ)
-structure var    (σ I V : Type*) := (stream : stream σ I V) (value : V) (init : σ)
-namespace iter
-variables {σ I V : Type} (a : iter σ I V) (s t : σ) [linear_order I]
+  (δ' : function.End σ) (ι' : σ → I) (ν' : σ → V) (ready' : σ → bool)
+structure stream (σ I V : Type*) extends iter σ I V :=  (q : σ)
+-- stream with a mutable value and upper bound; represents transient state of nested streams
+structure var    (σ I V : Type*) extends stream σ I V := (value : V) (init : σ) (size : ℕ)
+instance iter.functor {σ I} : functor (iter σ I) :=
+{map := λ {α β : Type} (f : α → β) (i : iter σ I α) , { i with ν' := f ∘ iter.ν' i } }
+instance stream.functor {σ I} : functor (stream σ I) := {map := λ {α β : Type} f s, { s with to_iter := f <$> s.to_iter } }
+instance var.functor {σ I} : functor (var σ I) := {
+  map := λ {α β : Type} (f : α → β) (v : var σ I α), {v with to_stream := f <$> v.to_stream, value := f v.value} }
+/- namespace -/ namespace iter
+variables {σ I V : Type*} (a : iter σ I V) (s t : σ)
+@[simp] def δ := a.δ' s
+@[simp] def ι := a.ι' s
+@[simp] def ν := a.ν' s
+@[simp] def ready := a.ready' s
 def reachable := relation.refl_trans_gen (λ s t, t = a.δ s)
-def monotonic := ∀ (s t : σ), a.reachable s t → a.ι s ≤ a.ι t
+variable [linear_order I]
+def monotonic := ∀ (s t : σ), a.reachable s t → a.ι' s ≤ a.ι' t
 end iter
-namespace stream
+/- namespace -/ namespace stream
 variables {σ I V : Type} (s : stream σ I V)
-@[simp] def δ (s : stream σ I V) : stream σ I V := { q := s.iter.δ s.q .. s}
-@[simp] def ι := s.iter.ι s.q @[simp] def ν := s.iter.ν s.q
-@[simp] def ready := s.iter.ready s.q
-variables [decidable_eq I] [has_top I] variables [add_monoid V]
-def elementary (i : I) (v : V) := λ j, if i = j then v else 0
-@[simp] def semantics₁  : I → V := if s.ready && (s.ι ≠ ⊤) then elementary s.ι s.ν else 0
-@[simp] def semantics : stream σ I V → ℕ → I → V | _ 0 := 0
-| s (n+1) := s.semantics₁ + semantics s.δ n
-notation `⟦` s, i `⟧` := s.semantics i
+@[simp] def δ (s : stream σ I V) : stream σ I V := { s with q := s.δ' s.q}
+@[simp] def ι := s.ι' s.q
+@[simp] def ν := s.ν' s.q
+@[simp] def ready := s.ready' s.q
+variables [decidable_eq I] [has_top I] [add_monoid V]
+--@[simp] def semantics₁  : I → V := if s.ready && (s.ι ≠ ⊤) then elementary s.ι s.ν else 0
+--@[simp] def semantics : stream σ I V → ℕ → I → V | _ 0 := 0
+--| s (n+1) := s.semantics₁ + semantics s.δ n
+--notation `⟦` s, k `⟧` := s.semantics k
 variables [linear_order I]
-@[simp] def monotonic := s.iter.monotonic
+@[simp] def monotonic := s.to_iter.monotonic
 end stream
-namespace var -- stream with a mutable value; represents transient state of nested streams
+class to_array (α : Type) (β : out_param Type) := (arrange : α → β)
+/- namespace -/ namespace var
 variables {σ I V : Type} (s : var σ I V)
-def δ : var σ I V := { s with stream := s.stream.δ, value := s.stream.δ.ν }
-@[simp] def ι := s.stream.ι @[simp] def ν := s.value
-def reset : var σ I V := { s with stream := { s.stream with q := s.init } }
+def δ : var σ I V := { s with to_stream := s.to_stream.δ, value := s.to_stream.δ.ν, size := s.size.decr }
+@[simp] def ι := s.to_stream.ι
+@[simp] def ν := s.value
+def reset : var σ I V := { s with to_stream := { s with q := s.init } }
+variables [decidable_eq I]
+@[simp] def semantics₁ [add_monoid V] : I → V := if s.to_stream.ready then elementary s.ι s.ν else 0
+@[simp] def semantics' [add_monoid V] : var σ I V → ℕ → I → V | _ 0 := 0
+| v (n+1) := v.semantics₁ + v.δ.semantics' n
+@[simp] def semantics [add_monoid V] (v : var σ I V) : I → V := v.semantics' v.size
+instance scalar.to_array [add_monoid V] : to_array V V := ⟨id⟩
+def arrange {V'} [add_monoid V'] [to_array V V'] : (var σ I V) → (I → V') :=
+λ v, (to_array.arrange <$> v).semantics
+structure var_state (σ V : Type*) := (value : V) (init : σ) (size : ℕ)
+-- def bounded_mutable_stream (σ I V : Type*) := stream (σ × var_state σ V) I V
+instance to_array {V'} [add_monoid V'] [to_array V V'] : to_array (var σ I V) (I → V') :=
+{ arrange := var.arrange }
+notation `⟦` v `⟧` := to_array.arrange v
 end var
-variable (v : var ℕ ℕ (var ℕ ℕ ℕ))
+
+--def flatten {σ₁ I₁ σ₂ I₂} : stream σ₁ I₁ (stream σ₂ I₂ V) → stream
+
+variables (v1 : var ℕ ℕ (var ℕ ℕ ℕ))
+#check v1.δ.arrange
+#check ⟦v1.δ⟧
+
+inductive BinOp | add | mul | lt | eq | and | or | min
+inductive LVal (γ : list Type) : Type → Type 1
+| ident {i} : hmem i γ → LVal i
+| value {σ I V : Type}   : LVal (var σ I V) → LVal V
 inductive E (γ : list Type) : Type → Type 1
 | ident {i} : hmem i γ → E i
-| value   {σ I V : Type} : E (var σ I V) → E V
+| value {σ I V : Type}   : E (var σ I V) → E V
 | current {σ I V : Type} : E (var σ I V) → E I
+| ready {σ I V : Type}   : E (var σ I V) → E bool
+| empty {σ I V : Type}   : E (var σ I V) → E bool
+| tt : E bool
+| ff : E bool
+--| bin_op : BinOp → E → E → E
+variable {γ : list Type}
 -- lens:
-def E.get {γ : list Type} (s : hlist γ) : Π {i}, E γ i → i
+def E.get (s : hlist γ) : Π {i}, E γ i → i
 | _ (E.ident var) := s.get var
 | _ (E.value e)   := e.get.ν
 | _ (E.current e) := e.get.ι
-def E.put {γ : list Type} (s : hlist γ) : Π {i}, E γ i → i → hlist γ
+| _ (E.ready e)   := e.get.to_stream.ready
+| _ (E.empty e)   := e.get.size = 0
+| _ (E.tt) := tt
+| _ (E.ff) := ff
+def E.put (s : hlist γ) : Π {i}, E γ i → i → hlist γ
 | _ (E.ident var) := λ v, s.update v var
-| _ (E.value e) := λ v, e.put { e.get s with value := v }
+| _ (E.value e)   := λ v, e.put { e.get s with value := v }
 | _ (E.current e) := λ _, s -- no
+| _ (E.empty e)   := λ _, s -- no
+| _ (E.ready e)   := λ _, s -- no
+| _ (E.tt) := λ _, s -- no
+| _ (E.ff) := λ _, s -- no
 def label := string
 inductive Prog (γ : list Type) : Type 1
 | expr {i} (e : E γ i) : Prog
@@ -53,16 +110,243 @@ inductive Prog (γ : list Type) : Type 1
 | seq (a b : Prog) : Prog
 | skip : Prog
 | jump : label → Prog
+| «if» : E γ bool → Prog → Prog → Prog
 infixr ` <;> `:1 := Prog.seq
+variables {σ I V : Type} (s : var σ I V)
+@[simp] def E.next (x : E γ (var σ I V)) : Prog γ := Prog.next x
+structure Gen (γ : list Type) (ι α : Type*) :=
+(current : ι)
+(value : α)
+(ready : E γ bool)
+(empty : E γ bool)
+(next (ifEmpty : unit → Prog γ) (ifNonempty : Prog γ → Prog γ) : Prog γ)
+(reset : Prog γ)
+(initialize : Prog γ)
+
+-- @[derive [decidable_eq, fintype]]
+-- def BinOp.mk_type : BinOp → Type 1
+-- | (BinOp.add) := Π{γ} {i: Type}, E γ i → E γ i → E γ i
+-- | (BinOp.mul) := Π{γ} {i: Type}, E γ i → E γ i → E γ i
+-- | (BinOp.lt)  := Π{γ} {i: Type}, E γ i → E γ i → E γ bool
+-- | (BinOp.eq)  := Π{γ} {i: Type}, E γ i → E γ i → E γ bool
+-- | (BinOp.and) := Π{γ} {i: Type}, E γ bool → E γ bool → E γ bool
+-- | (BinOp.or)  := Π{γ} {i: Type}, E γ bool → E γ bool → E γ bool
+-- | (BinOp.min) := Π{γ} {i: Type}, E γ i → E γ i → E γ i
+
+-- def BinOp.mk : Π (b : BinOp), BinOp.mk_type b
+-- | BinOp.and := λ γ i x y,
+--   match x, y with
+--   | E.tt, y := y
+--   | x, E.tt := x
+--   | x, y := E.bin_op BinOp.and x y
+--   end
+-- | BinOp.or := λ x y,
+--   match x, y with
+--   | E.false, y := y
+--   | x, E.false := x
+--   | E.true, _ := E.true
+--   | _, E.true := E.true
+--   | x, y := E.bin_op BinOp.or x y
+--   end
+-- | b := E.bin_op b
+-- instance : has_coe_to_fun BinOp BinOp.mk_type := ⟨BinOp.mk⟩
+
+-- def mulGen [has_mul α] (a b : Gen γ (E γ I) α) : Gen γ (E γ I) α :=
+-- { current := BinOp.min a.current b.current,
+--   value := a.value * b.value,
+--   ready := BinOp.eq a.current b.current && a.ready && b.ready,
+--   empty := a.empty || b.empty,
+--   next := λ kn ks, Prog.if (a.empty || b.empty) (kn ()) $
+--     Prog.if (BinOp.lt a.current b.current) (a.next kn ks) (b.next kn ks),
+--   reset := a.reset <;> b.reset,
+--   initialize := a.initialize <;> b.initialize }
+
 namespace Prog
 def blocks (γ : list Type) := label → Prog γ
-def step (γ : list Type) (s : hlist γ) (b : blocks γ) : Prog γ → (Prog γ × hlist γ)
+@[reducible] def state (γ : list Type) := Prog γ × hlist γ
+def step (b : blocks γ) (s : hlist γ) : Prog γ → (Prog γ × hlist γ)
 | (next e) := (skip, e.put s (e.get s).δ)
 | (store dst src) := (skip, dst.put s (src.get s))
 | (accum f dst src) := (skip, dst.put s $ f (dst.get s) (src.get s))
 | (skip <;> b) := (b, s)
 | (a <;> b) := let (a', s') := a.step in (a' <;> b, s')
 | (jump l) := (b l, s)
-| skip := (skip, s)
+| («if» c t e) := (if c.get s then t else e, s)
+| (skip) := (skip, s)
 | (expr _) := (skip, s) -- todo?
+def reachable {γ} (b : blocks γ) : state γ → state γ → Type* :=
+reduces (λ (p t : state γ), t = Prog.step b p.2 p.1)
+variables (prog : blocks γ)
+example (s : Prog γ × hlist γ) : reachable prog s s := reduces.refl
 end Prog
+
+section semantics
+variables (prog : Prog.blocks γ)
+
+def externGen {σ} {γ} (x : E γ (var σ I V)) : Gen γ (E γ I) (E γ V) :=
+{ current    := x.current,
+  value      := x.value,
+  ready      := E.tt,
+  empty      := x.empty,
+  next       := λ kn ks, Prog.if x.empty (kn ()) (ks x.next),
+  reset      := sorry, -- Prog.expr $ call "reset",
+  initialize := Prog.skip }
+
+def var_iter (x : E γ (var σ I V)) : iter (hlist γ) I V :=
+{ δ' := λ s, if x.empty.get s then s else (x.next.step prog s).2,
+  ι' := λ s, x.current.get s,
+  ν' := λ s, x.value.get s,
+  ready' := λ _, tt
+}
+
+def implements {σ : Type*} (g : Gen γ (E γ I) (E γ V)) (s : iter σ I V)
+(st : hlist γ) (st' : σ) : Prop
+:= (g.current.get st = s.ι st')
+∧  (g.ready.get st = s.ready st')
+∧  (s.ready st' → g.value.get st = s.ν st')
+def reachable_state {γ : list Type} (prog : Prog.blocks γ) (p : Prog γ) (s s' : hlist γ) : Prop :=
+nonempty (Prog.reachable prog (p,s) (p,s'))
+def simulates {σ : Type*} (g : Gen γ (E γ I) (E γ V)) (i : iter σ I V) (loop done : label)
+(st : hlist γ) (st' : σ) : Prop := implements g i st st' → ∃ st'' : hlist γ,
+reachable_state /-no-/prog
+  (g.next (λ _, Prog.jump done) (<;> Prog.jump loop))
+  st st'' ∧
+implements g i st'' st'
+
+
+def extend {α β} [decidable_eq α] (m : α → β) (k : α) (v : β) := λ k', if k = k' then v else m k'
+notation m `⟦` k `↦` v `⟧` := extend m k v
+
+def loopGen {γ : list Type} (loop done : label) (g : Gen γ (E γ I) (E γ V)) :=
+g.next (λ _, Prog.jump done) (<;> Prog.jump loop)
+
+def loopGenProg {γ : list Type} (prog : Prog.blocks γ) (loop done : label) (g : Gen γ (E γ I) (E γ V)) :=
+prog⟦loop ↦ loopGen loop done g⟧⟦done ↦ Prog.skip⟧
+
+theorem extern_sound (x : E γ (var σ I V)) (st : hlist γ) :
+implements (externGen x) (var_iter prog x) st st := begin
+simp [implements, externGen, var_iter, E.get],
+end
+
+lemma get_put {st : hlist γ} {α : Type} {y} (v : α) : (E.ident y).get ((E.ident y).put st v) = v := begin
+simp only [E.get, E.put, hlist.update, hlist.get],
+rw hlist.get_update,
+end
+lemma get_put_value {st : hlist γ} {α β : Type} (e : E γ (var α β V)) (v : V) : e.value.get (e.value.put st v) = v := begin
+simp only [E.get, E.put, hlist.update, hlist.get, stream.ν],
+sorry,
+end
+
+lemma var_form {α β : Type} (x : E γ (var σ I V)) : (∃ n, x = E.ident n) ∨ (∃ e : E γ (var α β (var σ I V)), x = e.value) := sorry
+
+theorem extern_step_sound (x : E γ (var σ I V)) (st : hlist γ) (loop done : label) :
+loop ≠ done → x.empty.get st = ff →
+∃ st' : hlist γ,
+reachable_state (loopGenProg prog loop done $ externGen x) (loopGen loop done $ externGen x) st st' ∧
+x.get st' = (x.get st).δ :=
+begin
+  intros neq hnonempty,
+  existsi _,
+  split,
+  { simp [reachable_state, loopGen, loopGenProg, externGen],
+    apply nonempty.intro,
+    apply reduces.tail,
+    simp only [Prog.step],
+    rw hnonempty, simp,
+    apply reduces.tail,
+    simp only [Prog.step],
+    apply reduces.tail,
+    simp only [Prog.step],
+    apply reduces.tail,
+    simp only [Prog.step, extend],
+    simp only [if_true, eq_self_iff_true],
+    split_ifs, {exfalso, exact neq h.symm},
+    exact reduces.refl,
+  },
+  cases var_form x,
+  { rw h.some_spec,
+    rw [get_put],
+  },
+  { rw h.some_spec,
+    rw [get_put_value], -- not correct
+    exact ℕ, -- hmm
+    exact ℕ,
+  },
+end
+
+example : Gen γ (E γ I) (E γ V) → var (Prog γ × hlist γ) I V := sorry
+
+variables {σ₁ σ₂ I₁ I₂ V₁ V₂ V₃ : Type} [linear_order I] [linear_order I₁] [linear_order I₂] (a : iter σ₁ I V₁) (b : iter σ₂ I V₂)
+variable (mul : V₁ → V₂ → V₃)
+
+variable (mulGen {γ γ'} (a : Gen γ (E γ I) (E γ V₁)) (b : Gen γ' (E γ' I) (E γ' V₂))
+: Gen (γ++γ') (E (γ++γ') I) (E (γ++γ') V₃))
+--variable (mulGen (a : Gen γ (E γ I) (E γ V₁)) (b : Gen γ (E γ I) (E γ V₂)) : Gen γ (E γ I) (E γ V₃))
+
+def mul_iter (a : iter σ₁ I V₁) (b : iter σ₂ I V₂) : iter (σ₁×σ₂) I V₃ :=
+{ δ' := λ ⟨s,t⟩, if a.ι s < b.ι t then (a.δ s,t) else if a.ι s > b.ι t then (s, b.δ t) else (a.δ s, b.δ t),
+  ι' := λ ⟨s,t⟩, min (a.ι s) (b.ι t),
+  ν' := λ ⟨s,t⟩, mul (a.ν s) (b.ν t),
+  ready' := λ ⟨s,t⟩, (a.ι s) = (b.ι t),
+}
+
+def mk_mul (a : stream σ₁ I V₁) (b : stream σ₂ I V₂) : stream (σ₁×σ₂) I V₃ :=
+⟨ mul_iter mul a.to_iter b.to_iter, (a.q, b.q) ⟩
+
+theorem mul_step_sound {γ'} (st : hlist γ) (st' : hlist γ') (σs σt : σ) (loop done : label)
+(prog : Prog.blocks (γ ++ γ'))
+(a : Gen γ  (E γ I) (E γ V₁))
+(b : Gen γ' (E γ' I) (E γ' V₂))
+(s : iter σ I V₁)
+(t : iter σ I V₂)
+-- (ha : implements a s st σs)
+-- (hb : implements b t st' σt)
+:
+loop ≠ done →
+∃ st'' : hlist (γ ++ γ'),
+reachable_state (loopGenProg prog loop done $ mulGen a b) (loopGen loop done $ mulGen a b) (st.append st') st'' ∧
+sorry = (mk_mul (s.get st) (t.get st')).δ /- extract state of (mulGen a b) from st'', compare to -/
+:=
+begin
+
+end
+
+#check @mulGen
+def mul_sound {γ'} {st : hlist γ} {st' : hlist γ'} {σs σt : σ}
+(a : Gen γ (E γ I) (E γ V₁)) (s : iter σ I V₁)
+(b : Gen γ (E γ I) (E γ V₂)) (t : iter σ I V₂)
+(ha : implements a s st σs)
+(hb : implements b t st σt) :
+implements (mulGen a b) (mul_iter mul s t) st (σs, σt) := begin
+split,
+simp [implements, mulGen, mul_iter, E.get],
+
+end
+
+end semantics
+
+namespace Prog
+attribute [refl] reduces.refl
+variables {r : α → α → Prop} {a b c : α}
+@[trans] def trans (hab : reduces r a b) (hbc : reduces r b c) : reduces r a c :=
+begin
+  induction hab generalizing c,
+  case reduces.refl { assumption },
+  case reduces.tail : d e f rde hef h { exact reduces.tail rde (h hbc) }
+end
+end Prog
+
+-- . update on component.
+-- empty → reduces to skip
+-- create LVal type?
+-- step_block_lemma?
+-- store as a Prop?
+
+/-
+σ → σ
+σ → (I → V) × σ
+σ → exp(σ, σ)
+σ → _ × exp(σ, σ)
+σ → F σ
+F t := t × (I → V) × I (× bool ?)
+-/
